DMC3.lean: some compositionality lemmas

Bakery/DMC3.lean
@@ -1,38 +1,138 @@
-import Mathlib.Logic.Relation
+--import Mathlib.Logic.Relation
+import Mathlib.Order.Lattice
 
 universe u
 
 -- this is merely a marker class i.e. empty fields
 class State (α : Type u) where
 
+
+/-
+  **Pattern α** : α → Prop
+-/
+
 abbrev Pattern (α : Type u) [State α] := α → Prop
 
--- TODO: define ↑ from State to Pattern
+-- ⊔ for Patterns
+def joinP {α : Type u} [State α] (p1 p2 : Pattern α) : Pattern α :=
+  fun st => p1 st ∨ p2 st
 
+instance {α : Type u} [State α] : Max (Pattern α) where
+  max := joinP
+
+-- define ↑ from State to Pattern
+def stateUp {α : Type u} [State α] : α → Pattern α :=
+  fun st => fun st' => st' = st
+
+instance {α : Type u} [State α] : Coe α (Pattern α) where
+  coe := stateUp
+
+
+/-
+  **Transition α** : α → α → Prop
+-/
 -- (inductively defined) set of rules (i.e. Rewrite Theory)
 abbrev Transition (α : Type u) [State α] := α → α → Prop
 
--- ⊔ for Transition for modular specification
+-- ⊔ for Transitions
 def joinT {α : Type u} [State α] (t1 t2 : Transition α) : Transition α :=
   fun st st' => t1 st st' ∨ t2 st st'
 
--- notation t1 "⊔" t2 => joinT t1 t2 (fix this reserved notation)
+instance {α : Type u} [State α] : Max (Transition α) where
+  max := joinT
 
 
 
--- Pattern → Pattern → Prop
-abbrev PTransition (α : Type u) [State α] := (α → Prop) → (α → Prop) → Prop
+/-
+  **Transformer α** : Pattern α → Pattern α → Prop
+  (Note) The term "transformer" may be misleading: it is a relation, not a function
+-/
+abbrev Transformer (α : Type u) [State α] := (α → Prop) → (α → Prop) → Prop
 
 -- (α → α → Prop) → ( (α → Prop) → (α → Prop) → Prop )
-def stepUp {α : Type u} [State α] : Transition α → PTransition α :=
+def stepUp {α : Type u} [State α] : Transition α → Transformer α :=
   fun t => fun p p' => ∀ st st', p st → t st st' → p' st'
 
---- System: State α with transition relation on α
+instance {α : Type u} [State α] : Coe (Transition α) (Transformer α) where
+  coe := stepUp
+
+-- ⊔ for Transformers
+def joinPT {α : Type u} [State α] (t1 t2 : Transformer α) : Transformer α :=
+  fun p p' => t1 p p' ∨ t2 p p'
+
+instance {α : Type u} [State α] : Max (Transformer α) where
+  max := joinPT
+
+-- ⊓ for Transformers
+def meetPT {α : Type u} [State α] (t1 t2 : Transformer α) : Transformer α :=
+  fun p p' => t1 p p' ∧ t2 p p'
+
+instance {α : Type u} [State α] : Min (Transformer α) where
+  min := meetPT
+
+
+/-
+  System
+-/
 class System (α : Type u) [State α] where
-  step : α → α → Prop
+  step : Transition α
 
--- structure Pattern (α : Type u) [State α] where
---   cond : α → Prop
 
--- def PStep (α : Type u) [State α] [System α] (p : Pattern α) (p' : Pattern α) : Prop :=
---   ∀ st st' : α, p.cond st → System.step st st' → p'.cond st'
+
+
+
+/- Decomposition rule for transformers (bidirectional)
+        p ⇒₁ p'     p ⇒₂ p'
+      ======================= (TransComp)
+          p (⇒₁ ⊔ ⇒₂) p'
+-/
+lemma TransComp {α : Type u} [State α] (t1 t2 : Transition α) (p p' : Pattern α) :
+  (↑(t1 ⊔ t2) : Transformer α) p p' ↔ (↑t1 : Transformer α) p p' ∧ (↑t2 : Transformer α) p p' := by
+  constructor
+  -- If "joined" post-image of p is in p', then so are "individual" post-images
+  · intro h
+    exact ⟨fun st st' hp ht1 => h st st' hp (Or.inl ht1),
+           fun st st' hp ht2 => h st st' hp (Or.inr ht2)⟩
+  -- If "individual" post-images of p are in p', then so is the "joined" post-image
+  · rintro ⟨h1, h2⟩ st st' hp (ht1 | ht2)
+    · exact h1 st st' hp ht1
+    · exact h2 st st' hp ht2
+
+-- ↑(t1 ⊔ t2) = ↑t1 ⊓ ↑t2
+-- To prove post-image safety w.r.t. a set of rules, we may decompose the proof into smaller pieces
+lemma TransComp_eq {α : Type u} [State α] (t1 t2 : Transition α) :
+  (↑(t1 ⊔ t2) : Transformer α) = (↑t1 : Transformer α) ⊓ (↑t2 : Transformer α) := by
+  ext p p' -- using function extensionality axiom
+  exact TransComp t1 t2 p p'
+
+/- Decomposition rule for pre-conditions (bidirectional)
+        p1 ⇒ p     p2 ⇒ p
+      ====================== (PreComp)
+          p1 ⊔ p2 ⇒ p
+-/
+lemma PreComp {α : Type u} [State α] (t : Transition α) (p p1 p2 : Pattern α) :
+  (↑t : Transformer α) (p1 ⊔ p2) p ↔ (↑t : Transformer α) p1 p ∧ (↑t : Transformer α) p2 p := by
+  constructor
+  -- Forward (->): If it's safe from the union, it's safe from each individual part
+  · intro h
+    exact ⟨fun st st' hp1 ht => h st st' (Or.inl hp1) ht,
+           fun st st' hp2 ht => h st st' (Or.inr hp2) ht⟩
+
+  -- Backward (<-): If it's safe from both parts, it's safe from the union
+  · rintro ⟨h1, h2⟩ st st' (hp1 | hp2) ht
+    · exact h1 st st' hp1 ht
+    · exact h2 st st' hp2 ht
+
+/- Decomposition rule for post-conditions (unidirectional)
+          p ⇒ p1
+      ----------------- (PostComp)
+        p ⇒ p1 ⊔ p2
+-/
+lemma PostComp {α : Type u} [State α] (t : Transition α) (p p1 p2 : Pattern α) :
+  (↑t : Transformer α) p p1 ∨ (↑t : Transformer α) p p2 → (↑t : Transformer α) p (p1 ⊔ p2) := by
+  -- Assume one of the transitions is strictly guaranteed
+  rintro (h1 | h2) st st' hp ht
+  -- Case 1: t guarantees p1
+  · exact Or.inl (h1 st st' hp ht)
+  -- Case 2: t guarantees p2
+  · exact Or.inr (h2 st st' hp ht)
